Prove the soundness of a transformation using bitmap index

fiat2/src/fiat2/BitmapIndex.v
@@ -67,6 +67,14 @@ Section WithHole.
     Definition pk_idx_wf (tbl_v idx_v : value) : Prop :=
       idx_v = interp_expr map.empty (map.put map.empty hole tbl_v) to_pk_idx.
 
+    Lemma to_pk_idx_wf : forall (v : value) (t : type),
+        type_wf t -> is_pk_tbl_ty t = true ->
+        type_of_value v t ->
+        pk_idx_wf v (interp_expr map.empty (map.put map.empty hole v) to_pk_idx).
+    Proof.
+      intros; unfold pk_idx_wf; auto.
+    Qed.
+
     Fixpoint mk_ids (n : nat) : list value :=
       match n with
       | O => []
@@ -323,8 +331,7 @@ End WithHole.
 Section WithHole.
   Context (attr str : string).
   Context (hole : string).
-  Context (tup acc : string).
-  Context (H_NoDup : is_NoDup_opaque [tup; acc]).
+  Context (tup : string).
 
   Definition to_bitmap :=
     EFlatmap LikeList (EVar hole) tup
@@ -369,34 +376,631 @@ Section WithHole.
     Definition bitmap_wf (tbl_v idx_v : value) : Prop :=
       idx_v = interp_expr map.empty (map.put map.empty hole tbl_v) to_bitmap.
 
+    Lemma to_bitmap_wf : forall (v : value) (t : type),
+        type_wf t -> is_bitmap_tbl_ty t = true ->
+        type_of_value v t ->
+        bitmap_wf v (interp_expr map.empty (map.put map.empty hole v) to_bitmap).
+    Proof.
+      intros; unfold bitmap_wf; auto.
+    Qed.
 
 
-  Context (x1 x2 b : string).
-  Context (EFlatmap2 : expr -> expr -> string -> string -> expr -> expr).
+    Definition bitmap_chara (tbl_v idx_v : value) : Prop :=
+      idx_v = match tbl_v with
+              | VList l1 =>
+                  VList
+                    (flat_map
+                       (fun v : value =>
+                          [VBool
+                             (value_eqb
+                                match v with
+                                | VRecord l => record_proj attr l
+                                | _ => VUnit
+                                end (VString str))]) l1)
+              | _ => VUnit
+              end.
 
-  Definition and_bitmaps bm1 bm2 :=
-      EFlatmap2 (EVar bm1) (EVar bm2)
-        x1 x2 (EBinop OCons (EBinop OAnd (EVar x1) (EVar x2)) (EAtom (ANil None))).
-
-  Definition use_bitmap bm d :=
-    let n := EAccess (EVar acc) "0" in
-    let l := EAccess (EVar acc) "1" in
-    EFold bm (ERecord [("0", EAtom (AInt 0)); ("1", EAtom (ANil None))])
-      b acc (ERecord [("0", EBinop OPlus n (EAtom (AInt 1)));
-                      ("1", EIf (EVar b) (EBinop OCons (EBinop OLookup d n) l) l)]).
-
-  Definition and_filter_to_bitmap_lookup_head (e : expr) bm1 bm2 :=
-    match e with
-    | EFilter LikeList (ELoc tbl0) x0 (EBinop OAnd (EBinop OEq (EAccess (EVar x1) attr0) str0)
-                                         (EBinop OEq (EAccess (EVar x2) attr1) str1)) =>
-        let n := EAccess (EVar acc) "0" in
-        let l := EAccess (EVar acc) "1" in
-        EAccess
-          (EFold (and_bitmaps bm1 bm2) (ERecord [("0", EAtom (AInt 0)); ("1", EAtom (ANil None))])
-           tup acc
-           (ERecord [("0", EBinop OPlus n (EAtom (AInt 1))); ("1", EBinop OCons (EBinop OLookup (ELoc tbl0) n) l)]))
-          "1"
-    | _ => e
-    end.
+    Lemma bitmap_wf__bitmap_chara : forall tbl_v idx_v,
+        bitmap_wf tbl_v idx_v ->
+        bitmap_chara tbl_v idx_v.
+    Proof.
+      unfold bitmap_wf, bitmap_chara; intros; subst.
+      cbn; unfold get_local; rewrite_map_get_put_goal.
+      case_match; auto. f_equal.
+      apply In_flat_map_ext; intros.
+      repeat f_equal. rewrite_map_get_put_goal.
+      reflexivity.
+    Qed.
   End WithMap.
 End WithHole.
+
+Section WithTags.
+  Context (id_tag aux_tag pk_idx_tag bm_tag : string).
+
+  Section filter_to_bitmap_lookup.
+    Context (tbl attr str : string).
+    Context (x1 b acc : string).
+    Context (H_NoDup : is_NoDup_opaque [x1; b; acc]).
+
+    Definition use_bitmap bm d :=
+      let n := EAccess (EVar acc) "0" in
+      let l := EAccess (EVar acc) "1" in
+      EFold bm (ERecord [("0", EAtom (AInt 0)); ("1", EAtom (ANil None))])
+        b acc (ERecord [("0", EBinop OPlus n (EAtom (AInt 1)));
+                        ("1", EIf (EVar b)
+                                (EOptMatch (EBinop OLookup d n)
+                                   l x1 (EBinop OCons (EVar x1) l))
+                                l)]).
+
+    Definition filter_to_bitmap_lookup_head (e : expr) :=
+      match e with
+      | EFilter LikeList (EAccess (ELoc tbl0) (id_tag0)) x
+          (EBinop OEq (EAccess (EVar x0) attr0) (EAtom (AString str0))) =>
+          if (all_eqb [(tbl, [tbl0]); (attr, [attr0]); (x, [x0; x1]); (id_tag, [id_tag0]); (str, [str0])])
+          then
+            let n := EAccess (EVar acc) "0" in
+            let l := EAccess (EVar acc) "1" in
+            EAccess
+              (use_bitmap
+                 (EAccess (EAccess (ELoc tbl) aux_tag) bm_tag)
+                 (EAccess (EAccess (EAccess (ELoc tbl) aux_tag) pk_idx_tag) "1"))
+              "1"
+          else e
+      | _ => e
+      end.
+
+    Section WithMap.
+      Context {tenv : map.map string type} {tenv_ok : map.ok tenv}.
+      Context {width: Z} {word: word.word width} {word_ok: word.ok word}.
+      Notation value := (value (width:=width)).
+      Context {locals : map.map string value} {locals_ok : map.ok locals}.
+
+      Lemma filter_to_bitmap_lookup_head_preserve_ty : forall tl t aux_tl (Gstore : tenv),
+          type_wf t -> is_pk_tbl_ty t = true ->
+          is_bitmap_tbl_ty attr t = true ->
+          map.get Gstore tbl = Some (TRecord tl) ->
+          access_record tl id_tag = Success t ->
+          access_record tl aux_tag = Success (TRecord aux_tl) ->
+          access_record aux_tl pk_idx_tag = Success (pk_idx_ty t) ->
+          access_record aux_tl bm_tag = Success (bitmap_ty t) ->
+          preserve_ty Gstore (filter_to_bitmap_lookup_head).
+      Proof.
+        unfold preserve_ty, is_pk_tbl_ty, is_bitmap_tbl_ty. intros.
+        repeat destruct_match_hyp; try congruence.
+        repeat destruct_subexpr. simpl.
+        case_match; auto. repeat rewrite Bool.andb_true_r in *.
+        repeat rewrite Bool.andb_true_iff in *; intuition idtac.
+        rewrite eqb_eq in *; subst.
+        repeat invert_type_of_clear. repeat invert_type_of_op_clear.
+        repeat rewrite_map_get_put_hyp.
+        repeat (clear_refl; repeat do_injection2).
+        repeat (rewrite_l_to_r; do_injection2).
+        econstructor.
+        1: econstructor.
+        1: repeat (econstructor; eauto).
+        1:{ lazymatch goal with
+            H: tenv_wf ?G, H': map.get ?G _ = _ |- _ =>
+              apply H in H'
+          end.
+            repeat invert_type_wf.
+            instantiate(1:=[("0", TInt); ("1", TList (TRecord tl0))]).
+            repeat (econstructor; eauto). cbn; intuition discriminate. }
+        1:{ repeat (econstructor; eauto);
+            repeat rewrite_map_get_put_goal; eauto;
+            use_is_NoDup. }
+        cbn; reflexivity.
+      Qed.
+
+      Context (pk_hole pk_tup pk_acc : string).
+      Context (H_NoDup_pk : is_NoDup_opaque [pk_tup; pk_acc]).
+
+      Notation pk_idx_wf := (pk_idx_wf pk_hole pk_tup pk_acc).
+
+      Definition aux_wf_for_idx idx_tag idx_wf (v : value) : Prop :=
+        match v with
+        | VRecord rv =>
+            match access_record rv id_tag with
+            | Success v_id =>
+                match access_record rv aux_tag with
+                | Success (VRecord rv_aux) =>
+                    match access_record rv_aux idx_tag with
+                    | Success v_idx =>
+                        idx_wf v_id v_idx
+                    | _ => False
+                    end
+              | _ => False
+              end
+          | _ => False
+          end
+        | _ => False
+        end.
+
+      Context (bm_hole : string).
+      Context (bm_tup : string).
+      Notation bitmap_wf := (bitmap_wf attr str bm_hole bm_tup).
+
+      (* ??? TODO: move *)
+      Lemma Forall2_access_record : forall A A' P l l' x (a : A) (a' : A'),
+          Forall2 (fun p p' => fst p = fst p' /\ P (snd p) (snd p')) l l' ->
+          access_record l x = Success a ->
+          access_record l' x = Success a' ->
+          P a a'.
+      Proof.
+        induction 1; cbn; try discriminate; auto.
+        repeat case_match; cbn in *; intuition idtac;
+          repeat (try clear_refl; do_injection); subst; auto;
+          congruence.
+      Qed.
+
+      Ltac use_Forall2_access_record tag :=
+        lazymatch goal with
+          H: Forall2 _ ?l ?tl, H1: access_record ?l tag = _,
+              H2: access_record ?tl tag = _ |- _ =>
+            pose proof (Forall2_access_record _ _ _ _ _ _ _ _ H H1 H2)
+        end.
+
+      Lemma fiat2_gallina_use_bitmap : forall (store env : locals) bm d,
+          free_immut_in b d = false ->
+          free_immut_in acc d = false ->
+          interp_expr store env (use_bitmap bm d) =
+            match interp_expr store env bm with
+            | VList l1 =>
+                fold_right
+                  (fun v acc0 : value =>
+                     VRecord
+                       [("0",
+                          apply_int_binop Z.add
+                            match
+                              acc0
+                            with
+                            | VRecord l => record_proj "0" l
+                            | _ => VUnit
+                            end (VInt 1));
+                        ("1",
+                          match
+                            v
+                          with
+                          | VBool true =>
+                              match
+                                match
+                                  interp_expr store env d
+                                with
+                                | VDict d0 =>
+                                    VOption
+                                      (dict_lookup
+                                         match
+                                           acc0
+                                         with
+                                         | VRecord l => record_proj "0" l
+                                         | _ => VUnit
+                                         end d0)
+                                | _ => VUnit
+                                end
+                              with
+                              | VOption (Some v0) =>
+                                  match
+                                    match acc0
+                                    with
+                                    | VRecord l => record_proj "1" l
+                                    | _ => VUnit
+                                    end
+                                  with
+                                  | VList l =>
+                                      VList
+                                        (v0 :: l)
+                                  | _ => VUnit
+                                  end
+                              | VOption None =>
+                                  match acc0
+                                  with
+                                  | VRecord l => record_proj "1" l
+                                  | _ => VUnit
+                                  end
+                              | _ => VUnit
+                              end
+                          | VBool false =>
+                              match acc0
+                              with
+                              | VRecord l => record_proj "1" l
+                              | _ => VUnit
+                              end
+                          | _ => VUnit
+                          end)]) (VRecord [("0", VInt 0); ("1", VList [])])
+                  l1
+            | _ => VUnit
+            end.
+      Proof.
+        intros; unfold use_bitmap; cbn.
+        case_match; auto.
+        apply In_fold_right_ext with (P:=fun _ => True); intuition idtac.
+        repeat f_equal; unfold get_local; repeat rewrite_map_get_put_goal; auto.
+        2: use_is_NoDup.
+        case_match; auto.
+        repeat rewrite_map_get_put_goal.
+        repeat rewrite <- not_free_immut_put_sem; auto.
+        repeat (case_match; auto; []).
+        do 2 case_match; auto; repeat rewrite_map_get_put_goal; auto.
+        all: use_is_NoDup.
+      Qed.
+
+      Lemma In_dict_lookup : forall (k v : value) d,
+          StronglySorted (fun v1 v2=> is_true (dict_entry_leb v1 v2)) d ->
+          NoDup (List.map fst d) ->
+          In (k, v) d ->
+          dict_lookup k d = Some v.
+      Proof.
+        induction d; cbn; intros.
+        1: intuition idtac.
+        case_match. case_match.
+        1:{ intuition idtac; try invert_pair; auto.
+            lazymatch goal with
+              H: value_eqb _ _ = true |- _ =>
+                apply value_eqb_eq in H
+            end; subst.
+            invert_NoDup.
+            lazymatch goal with
+              H: In _ _ |- _ =>
+                apply in_map with (f:=fst) in H
+            end. intuition idtac. }
+        1:{ lazymatch goal with
+            H: value_eqb _ _ = false |- _ =>
+              apply value_eqb_neq in H
+          end.
+            invert_NoDup; invert_SSorted; apply IHd; intuition auto.
+            congruence. }
+      Qed.
+
+      Lemma dict_lookup_Some__In : forall (k v : value) d,
+          dict_lookup k d = Some v -> In (k, v) d.
+      Proof.
+        induction d; cbn; try discriminate.
+        repeat case_match; intros; auto.
+        do_injection. apply value_eqb_eq in E0; subst; auto.
+      Qed.
+
+      Lemma is_pk_idx__dict_lookup : forall (l : list value) d,
+          is_pk_idx (mk_ids (Datatypes.length l)) l d ->
+          Forall2 (fun k v => dict_lookup k d = Some v) (mk_ids (Datatypes.length l)) l.
+      Proof.
+        unfold is_pk_idx; intros; subst.
+        induction l.
+        1: cbn; auto.
+        cbn [flat_map2 Datatypes.length mk_ids app].
+        constructor;
+          (assert (Heq: forall (k v : value) l l',
+                (k, v) :: flat_map2 (fun k v => [(k, v)]) l l' = flat_map2 (fun k v => [(k, v)]) (k :: l) (v :: l')); [ reflexivity | ];
+          assert (Heq': VInt (Z.of_nat (Datatypes.length l)) :: mk_ids (width:=width) (Datatypes.length l) = mk_ids (Datatypes.length (a :: l)));  [ reflexivity | ]).
+        1:{ apply In_dict_lookup; auto using StronglySorted_dict_sort.
+            1:{ eapply Permutation_NoDup.
+                1: eapply Permutation_map, Permuted_dict_sort.
+                rewrite Heq, Heq'.
+                rewrite map_fst_flat_map2_mk_ids.
+                apply mk_ids_NoDup. }
+            1:{ eapply Permutation_in.
+                1: apply Permuted_dict_sort.
+                constructor; reflexivity. } }
+        1:{ eapply Forall2_impl; eauto; simpl; intros.
+            apply In_dict_lookup; auto using StronglySorted_dict_sort.
+            1:{ eapply Permutation_NoDup.
+                1: eapply Permutation_map, Permuted_dict_sort.
+                rewrite Heq, Heq'.
+                rewrite map_fst_flat_map2_mk_ids.
+                apply mk_ids_NoDup. }
+            1:{ eapply Permutation_in.
+                1: apply Permuted_dict_sort.
+                right.
+                lazymatch goal with
+                  H: dict_lookup _ _ = Some _ |- _ =>
+                    apply dict_lookup_Some__In in H
+                end.
+                eapply Permutation_in; [ | eauto ].
+                apply Permutation_sym, Permuted_dict_sort. } }
+      Qed.
+
+      Lemma use_bitmap_sem : forall l d bm tl (store env : locals),
+          free_immut_in b d = false ->
+          free_immut_in acc d = false ->
+          match interp_expr store env d with
+          | VDict d =>
+              is_pk_idx (mk_ids (Datatypes.length l)) l d
+          | _ => False
+          end ->
+          bitmap_chara attr str (VList l) (interp_expr store env bm) ->
+          Forall (fun v : value => type_of_value v (TRecord tl)) l ->
+          access_record tl attr = Success TString ->
+          interp_expr store env (use_bitmap bm d) =
+            VRecord [("0", VInt (Z.of_nat (Datatypes.length l)));
+                     ("1", VList
+                             (filter (fun v =>
+                                        match v with
+                                        | VRecord r =>
+                                            match access_record r attr with
+                                            | Success v => value_eqb v (VString str)
+                                            | Failure _ => false
+                                            end
+                                        | _ => false
+                                        end) l))].
+      Proof.
+        unfold bitmap_chara. intros; cbn in * |-.
+        rewrite fiat2_gallina_use_bitmap; auto.
+        destruct_match_hyp; intuition idtac.
+        lazymatch goal with
+          H: is_pk_idx _ _ _ |- _ =>
+            apply is_pk_idx__dict_lookup in H
+        end.
+        rewrite_l_to_r. clear H2.
+        induction l.
+        1: cbn; auto.
+        cbn [flat_map app].
+        invert_Forall. invert_type_of_value_clear.
+        cbn [fold_right].
+        erewrite IHl; cbn; auto.
+        2:{ cbn in *. invert_Forall2; auto. }
+        repeat f_equal.
+        1:{ rewrite Zpos_P_of_succ_nat.
+            rewrite Z.add_1_r. reflexivity. }
+        1:{ apply access_record_sound in H4.
+            apply in_map with (f:=fst) in H4; cbn in H4.
+            lazymatch goal with
+                H: Forall2 (fun _ _ => _ /\ _) _ _ |- _ =>
+                  apply Forall2_split in H
+              end; intuition idtac.
+            apply Forall2_fst_eq in H2.
+            rewrite <- H2 in H4.
+            apply In_access_record in H4; destruct_exists.
+            unfold record_proj.
+            rewrite_l_to_r.
+            case_match; auto.
+            invert_Forall2. rewrite_l_to_r. reflexivity. }
+      Qed.
+
+      Lemma filter_to_bitmap_lookup_head_preserve_sem : forall (Gstore : tenv) (store : locals) tl t aux_tl,
+          type_wf t -> is_pk_tbl_ty t = true ->
+          is_bitmap_tbl_ty attr t = true ->
+          map.get Gstore tbl = Some (TRecord tl) ->
+          access_record tl id_tag = Success t ->
+          access_record tl aux_tag = Success (TRecord aux_tl) ->
+          access_record aux_tl pk_idx_tag = Success (pk_idx_ty t) ->
+          access_record aux_tl bm_tag = Success (bitmap_ty t) ->
+          match map.get store tbl with
+          | Some v => aux_wf_for_idx pk_idx_tag pk_idx_wf v /\
+                        aux_wf_for_idx bm_tag bitmap_wf v
+          | _ => False
+          end ->
+          preserve_sem Gstore store filter_to_bitmap_lookup_head.
+      Proof.
+        unfold preserve_sem, aux_wf_for_idx; intros.
+        repeat (destruct_match_hyp; try discriminate; intuition idtac; []).
+        eapply pk_idx_wf__pk_idx_chara in H13; eauto.
+        all: unfold is_pk_tbl_ty, is_bitmap_tbl_ty, pk_idx_ty, bitmap_ty in *.
+        all: apply_locals_wf store;
+          repeat (destruct_match_hyp; try discriminate; intuition idtac; []);  do_injection.
+        all: invert_type_of_value_clear;
+          use_Forall2_access_record id_tag; auto.
+        use_Forall2_access_record aux_tag.
+        invert_type_of_value_clear.
+        use_Forall2_access_record pk_idx_tag.
+        use_Forall2_access_record bm_tag.
+        repeat destruct_subexpr. unfold filter_to_bitmap_lookup_head.
+        case_match; auto. cbn in * |-.
+        repeat rewrite Bool.andb_true_iff in *; intuition idtac.
+        rewrite eqb_eq in *; subst. repeat clear_refl.
+        cbn [interp_expr interp_binop apply_bool_binop interp_atom].
+        unfold get_local. rewrite_l_to_r.
+        unfold record_proj. repeat rewrite_l_to_r.
+        repeat invert_type_of_value_clear.
+        rewrite type_eqb_eq in *; subst.
+        unfold pk_idx_chara in *.
+        destruct_and. repeat (destruct_match_hyp; intuition idtac).
+        erewrite use_bitmap_sem; try reflexivity.
+        4,5: eauto.
+        2:{ cbn. unfold get_local, record_proj; repeat rewrite_l_to_r.
+            eauto. }
+        2:{ eapply bitmap_wf__bitmap_chara; auto; cbn.
+            unfold get_local, record_proj; repeat rewrite_l_to_r. eauto. }
+        cbn. f_equal.
+        apply In_filter_ext; intros. apply_Forall_In.
+        invert_type_of_value_clear. rewrite_map_get_put_goal.
+        lazymatch goal with
+          H: Forall2 _ l6 _ |- _ => apply Forall2_split in H as [HL HR] end.
+        rewrite Forall2_fst_eq in HL.
+        lazymatch goal with
+          H: access_record l1 _ = _ |- _ =>
+            apply access_record_sound in H;
+            apply in_map with (f:=fst) in H; cbn in H;
+            rewrite <- HL in H; apply In_access_record in H
+        end.
+        destruct_exists; rewrite_l_to_r. reflexivity.
+      Qed.
+    End WithMap.
+
+  End filter_to_bitmap_lookup.
+
+End WithTags.
+
+(*
+    Context (tbl attr1 str1 attr2 str2 : string).
+    Context (x1 x2 b acc : string).
+    Context (H_NoDup : is_NoDup_opaque [x1; x2; b; acc]).
+
+    Definition and_bitmaps bm1 bm2 :=
+      EFlatmap2 bm1 bm2
+        x1 x2 (EBinop OCons (EBinop OAnd (EVar x1) (EVar x2)) (EAtom (ANil None))).
+
+    Definition use_bitmap bm d :=
+      let n := EAccess (EVar acc) "0" in
+      let l := EAccess (EVar acc) "1" in
+      EFold bm (ERecord [("0", EAtom (AInt 0)); ("1", EAtom (ANil None))])
+        b acc (ERecord [("0", EBinop OPlus n (EAtom (AInt 1)));
+                        ("1", EIf (EVar b)
+                                (EOptMatch (EBinop OLookup d n)
+                                   l x1 (EBinop OCons (EVar x1) l))
+                                l)]).
+
+    Definition and_filter_to_lookup_head (e : expr) :=
+      match e with
+      | EFilter LikeList (EAccess (ELoc tbl0) (id_tag0)) x
+          (EBinop OAnd (EBinop OEq (EAccess (EVar x0) attr1') str1')
+             (EBinop OEq (EAccess (EVar x1) attr2') str2')) =>
+          if (all_eqb [(tbl, [tbl0]); (attr1, [attr1']); (attr2, [attr2']); (x, [x0; x1]); (id_tag, [id_tag0])])
+          then
+            let n := EAccess (EVar acc) "0" in
+            let l := EAccess (EVar acc) "1" in
+            EAccess
+              (use_bitmap
+                 (and_bitmaps
+                    (EAccess (EAccess (ELoc tbl) aux_tag) bm1_tag)
+                    (EAccess (EAccess (ELoc tbl) aux_tag) bm2_tag))
+                 (EAccess (EAccess (EAccess (ELoc tbl) aux_tag) pk_idx_tag) "1"))
+              "1"
+          else e
+      | _ => e
+      end.
+
+  Section WithMap.
+    Context {tenv : map.map string type} {tenv_ok : map.ok tenv}.
+    Context {width: Z} {word: word.word width} {word_ok: word.ok word}.
+    Notation value := (value (width:=width)).
+    Context {locals : map.map string value} {locals_ok : map.ok locals}.
+
+    Lemma and_bitmaps_ty : forall Gstore Genv e1 e2,
+        type_of Gstore Genv e1 (TList TBool) ->
+        type_of Gstore Genv e2 (TList TBool) ->
+        type_of Gstore Genv (and_bitmaps e1 e2) (TList TBool).
+    Proof.
+      clear H_NoDup.
+      intros. econstructor; eauto.
+      repeat econstructor; try now (rewrite_map_get_put_goal; auto).
+      destruct_get_put_strings; auto.
+    Qed.
+
+    Lemma and_filter_to_lookup_head_preserve_ty : forall tl t aux_tl (Gstore : tenv),
+        type_wf t -> is_pk_tbl_ty t = true ->
+        is_bitmap_tbl_ty attr1 t = true ->
+        is_bitmap_tbl_ty attr2 t = true ->
+        map.get Gstore tbl = Some (TRecord tl) ->
+        access_record tl id_tag = Success t ->
+        access_record tl aux_tag = Success (TRecord aux_tl) ->
+        access_record aux_tl pk_idx_tag = Success (pk_idx_ty t) ->
+        access_record aux_tl bm1_tag = Success (bitmap_ty t) ->
+        access_record aux_tl bm2_tag = Success (bitmap_ty t) ->
+        preserve_ty Gstore (and_filter_to_lookup_head).
+    Proof.
+      unfold preserve_ty, is_pk_tbl_ty, is_bitmap_tbl_ty. intros.
+      repeat destruct_match_hyp; try congruence.
+      repeat destruct_subexpr. simpl.
+      case_match; auto. repeat rewrite Bool.andb_true_r in *.
+      repeat rewrite Bool.andb_true_iff in *; intuition idtac.
+      rewrite eqb_eq in *; subst.
+      repeat invert_type_of_clear. repeat invert_type_of_op_clear.
+      repeat rewrite_map_get_put_hyp.
+      repeat (clear_refl; repeat do_injection2).
+      repeat (rewrite_l_to_r; do_injection2).
+      econstructor.
+      1: econstructor.
+      1: apply and_bitmaps_ty; repeat (econstructor; eauto).
+      1:{ lazymatch goal with
+          H: tenv_wf ?G, H': map.get ?G _ = _ |- _ =>
+            apply H in H'
+        end.
+          repeat invert_type_wf.
+          instantiate(1:=[("0", TInt); ("1", TList (TRecord tl1))]).
+          repeat (econstructor; eauto). cbn; intuition discriminate. }
+      1:{ repeat (econstructor; eauto);
+          repeat rewrite_map_get_put_goal; eauto;
+          use_is_NoDup. }
+      cbn; reflexivity.
+    Qed.
+
+    Context (pk_hole pk_tup pk_acc : string).
+    Context (H_NoDup_pk : is_NoDup_opaque [pk_tup; pk_acc]).
+
+    Notation pk_idx_wf := (pk_idx_wf pk_hole pk_tup pk_acc).
+
+    Definition aux_wf_for_idx idx_tag idx_wf (v : value) : Prop :=
+      match v with
+      | VRecord rv =>
+          match access_record rv id_tag with
+          | Success v_id =>
+              match access_record rv aux_tag with
+              | Success (VRecord rv_aux) =>
+                  match access_record rv_aux idx_tag with
+                  | Success v_idx =>
+                      idx_wf v_id v_idx
+                  | _ => False
+                  end
+              | _ => False
+              end
+          | _ => False
+          end
+      | _ => False
+      end.
+
+    Context (bm1_hole bm2_hole : string).
+    Context (bm1_tup bm2_tup : string).
+    Notation bitmap1_wf := (bitmap_wf attr1 str1 bm1_hole bm1_tup).
+    Notation bitmap2_wf := (bitmap_wf attr2 str2 bm2_hole bm2_tup).
+
+    (* ??? TODO: move *)
+    Lemma Forall2_access_record : forall A A' P l l' x (a : A) (a' : A'),
+        Forall2 (fun p p' => fst p = fst p' /\ P (snd p) (snd p')) l l' ->
+        access_record l x = Success a ->
+        access_record l' x = Success a' ->
+        P a a'.
+    Proof.
+      induction 1; cbn; try discriminate; auto.
+      repeat case_match; cbn in *; intuition idtac;
+        repeat (try clear_refl; do_injection); subst; auto;
+        congruence.
+    Qed.
+
+    Ltac use_Forall2_access_record tag :=
+      lazymatch goal with
+        H: Forall2 _ ?l ?tl, H1: access_record ?l tag = _,
+            H2: access_record ?tl tag = _ |- _ =>
+          pose proof (Forall2_access_record _ _ _ _ _ _ _ _ H H1 H2)
+      end.
+
+    Lemma and_filter_to_lookup_head_preserve_sem : forall (Gstore : tenv) (store : locals) tl t aux_tl,
+        type_wf t -> is_pk_tbl_ty t = true ->
+        is_bitmap_tbl_ty attr1 t = true ->
+        is_bitmap_tbl_ty attr2 t = true ->
+        map.get Gstore tbl = Some (TRecord tl) ->
+        access_record tl id_tag = Success t ->
+        access_record tl aux_tag = Success (TRecord aux_tl) ->
+        access_record aux_tl pk_idx_tag = Success (pk_idx_ty t) ->
+        access_record aux_tl bm1_tag = Success (bitmap_ty t) ->
+        access_record aux_tl bm2_tag = Success (bitmap_ty t) ->
+        match map.get store tbl with
+        | Some v => aux_wf_for_idx pk_idx_tag pk_idx_wf v /\
+                      aux_wf_for_idx bm1_tag bitmap1_wf v /\
+                      aux_wf_for_idx bm2_tag bitmap2_wf v
+        | _ => False
+        end ->
+        preserve_sem Gstore store and_filter_to_lookup_head.
+    Proof.
+      unfold preserve_sem, aux_wf_for_idx; intros.
+      unfold is_pk_tbl_ty, is_bitmap_tbl_ty, pk_idx_ty, bitmap_ty in *.
+      apply_locals_wf store.
+      repeat (destruct_match_hyp; try discriminate; intuition idtac; []).
+
+      invert_type_of_value_clear.
+      use_Forall2_access_record id_tag.
+      use_Forall2_access_record aux_tag.
+      invert_type_of_value_clear.
+      use_Forall2_access_record pk_idx_tag.
+      use_Forall2_access_record bm1_tag.
+      use_Forall2_access_record bm2_tag.
+      repeat destruct_subexpr. unfold and_filter_to_lookup_head.
+      case_match; auto. cbn in * |-.
+      repeat rewrite Bool.andb_true_iff in *; intuition idtac.
+      rewrite eqb_eq in *; subst. repeat clear_refl.
+      unfold use_bitmap, and_bitmaps.
+      cbn [interp_expr interp_binop apply_bool_binop].
+      unfold get_local. rewrite_l_to_r.
+      unfold record_proj. repeat rewrite_l_to_r.
+      repeat invert_type_of_value_clear.
+
+
+  End WithMap.
+*)
